### 2 번

##### T(n) = T(n - 1) + n

`T(0) = 1` 로 설정



##### 풀이

T(n) = T(n-2) + n-1 + 1 = ... = T(1) + n * n + C (단, C는 상수) 

O(n^2)



### 4번

##### T(n) = T(n/2) + 1

`T(1) = 1`로 설정





##### 풀이

T(n) = T(n/2^2) + 2 = T(1) + k

k = log(n)으로 설정하면 T(n/2^k) = T(1)이므로

답은 O(log(n))



### 6번

##### T(n) = 2T(n/2) + n



##### 풀이

T(n) = 2^kT(n/2^k) + n + n + n +.... + n = 2^kT(n/2^k) + n*k

k = logn을대입 T(n) = n * T(1) + nlogn

답은 O(nlogn)



### 8번

##### T(n) = T(n - 1) + 1/n



##### 풀이

T(n-1) = T(n-2) + 1/n + 1/n-1 이므로

T(n) = T(1) + 1/n + 1/(n-1) + ... + 1/(n-k) = 1 + 1/2 + 1/3 + .... + 1/n이고

n이 무한대로 갈때 무한급수는 적분으로 변환가능하므로  logn + C임을 보이므로

답은 O(logn)이다.

